Validator/Validator/Validate.lean
@@ -24,7 +24,7 @@ import Validator.Validator.Inst.TreeParserMemM
 namespace Validate
 
 def deriveEnter [DecidableEq φ] [ValidateM m n φ α]
-  (G: Grammar n φ) (Φ: φ -> α -> Prop) [DecidableRel Φ]
+  (G: Grammar n φ) (Φ: φ -> α -> Bool)
   (xs: Rules n φ l): m (Rules n φ (Symbol.nums xs)) := do
   let token <- Parser.token
   let enters <- Enter.DeriveEnter.deriveEnter xs
@@ -34,12 +34,12 @@ def deriveLeaveM [ValidateM m n φ α] (xs: Rules n φ l) (cs: Rules n φ (Symbo
   Leave.DeriveLeaveM.deriveLeaveM xs (Vec.map cs Rule.nullable)
 
 def deriveValue [DecidableEq φ] [ValidateM m n φ α]
-  (G: Grammar n φ) (Φ: φ -> α -> Prop) [DecidableRel Φ]
+  (G: Grammar n φ) (Φ: φ -> α -> Bool)
   (xs: Rules n φ l): m (Rules n φ l) := do
   deriveLeaveM (α := α) xs (<- deriveEnter G Φ xs)
 
 partial def derive [DecidableEq φ] [ValidateM m n φ α]
-  (G: Grammar n φ) (Φ: φ -> α -> Prop) [DecidableRel Φ]
+  (G: Grammar n φ) (Φ: φ -> α -> Bool)
   (xs: Rules n φ l): m (Rules n φ l) := do
   if List.all xs.toList Regex.unescapable then
     Parser.skip; return xs
@@ -66,13 +66,13 @@ partial def derive [DecidableEq φ] [ValidateM m n φ α]
   | Hint.eof => return xs -- only happens at the top
 
 def validate {m} {n: Nat} {α: Type} [DecidableEq φ]
-  (G: Grammar n φ) (Φ: φ -> α -> Prop) [DecidableRel Φ]
+  (G: Grammar n φ) (Φ: φ -> α -> Bool)
   [ValidateM m n φ α] (x: Rule n φ): m Bool := do
   let dxs <- derive G Φ (Vec.cons x Vec.nil)
   return Rule.nullable dxs.head
 
 def run {α: Type} [DecidableEq α] [Hashable α] (G: Grammar n (Pred α)) (t: Hedge.Node α): Except String Bool :=
-  TreeParserMemM.run' (n := n) (φ := Pred α) (validate G Pred.eval G.start) t
+  TreeParserMemM.run' (n := n) (φ := Pred α) (validate G Pred.evalb G.start) t
 
 -- Tests
 
